Add proof for totalSupply.

src/dafny/yul-verif-examples/erc-20/erc-20.dfy
@@ -15,7 +15,7 @@
 include "../../Yul/Semantics.dfy"
 include "../../Yul/StrictSemantics.dfy"
 include "../../Yul/State.dfy"
-
+// include "../../../../libs/evm-dafny/src/dafny/util/bytes.dfy"
 
 
 /**
@@ -26,59 +26,211 @@ module ERC20 {
   import opened Int
   import opened YulSem = YulStrict
   import opened YulState
+  import ByteUtils
 
   datatype Either<A, B> = Left(val: A) | Right(error: B)
 
   predicate GInv(s: Executing)
   {
     true
+    // totalSupply ==
     //  some of balances should be total supply
   }
 
-  method Main(s: Executing) returns (s': State)
+
+  method Main(s: Executing, ghost totalSupply: u256) returns (s': State)
+    requires totalSupply == s.Load(0)
     requires s.MemSize() % 32 == 0
-
-    ensures CallValue(s) != 0 ==> s'.ERROR?
-    // ensures Memory.Size(m') > 0x40 + 31
-    // ensures Memory.ReadUint256(m', 0x40) == 8
+    requires 4 <= CallDataSize(s) as nat < TWO_255 - 4
+    ensures CallDataSize(s) < 4 ==> s'.ERROR?
+    ensures CallDataSize(s) >= 4 && shift_right_224_unsigned(CallDataLoad(0, s)) == 0x18160ddd ==> ByteUtils.ReadUint256(s'.data, 0) == s.Load(0)
+    ensures s'.RETURNS? ==> ByteUtils.ReadUint256(s'.data, 0) == totalSupply
   {
-    //  Non payable, callvalue must be zero, otherwise we revert.
-    if !IsZero((CallValue(s))) {
-      return Revert(0, 0, s);
+
+    // var s1 := MStore(64, MemoryGuard(128), s);
+    // assert s1.Read(64) == 128;
+    // assert CallDataSize(s1) == CallDataSize(s);
+    var s1 := s;
+
+    if !Lt(CallDataSize(s1), 4) {
+      //  There is enough calldata for a 4-byte selector
+      assert CallDataSize(s1) >= 4;
+      //  Extract selector
+      var selector := shift_right_224_unsigned(CallDataLoad(0, s1));
+      match selector
+
+      case 0x18160ddd =>
+        {
+          // totalSupply()
+
+          var s2 := external_fun_totalSupply_3(s1);
+          assert s2.RETURNS? ==> |s2.data| == 32; 
+          assert s2.RETURNS? ==> ByteUtils.ReadUint256(s2.data, 0) == s.Load(0);
+          return s2;
+        }
+
+      case 0xa0712d68 =>
+        {
+          // mint(uint256)
+
+          // external_fun_mint_13()
+          return s1;
+        }
+
+      case _ => return Revert(0, 0, s1);
+
     }
+    assert CallDataSize(s1) < 4;
+    return Revert(0, 0, s1);
+  }
 
-    s' := s;
+  /** Get leftmost 4-bytes of a u256. */
+  function shift_right_224_unsigned(value: u256): (newValue: u256)
+  {
+    Shr(224, value)
+  }
 
-    match selector(s)
-    case 0x70a08231 /* "balanceOf(address)" */ => {
-      // returnUint(balanceOf(decodeAsAddress(0)))
-      s' := s;
+  /** Get the free memory pointer. */
+  method allocate_unbounded(s: Executing) returns (memPtr: u256, s': State)
+    requires s.MemSize() % 32 == 0
+    ensures s'.EXECUTING?
+    ensures s'.MemSize() % 32 == 0
+  {
+    return MLoad(64, s).0, MLoad(64, s).1;
+  }
+
+  method revert_error_ca66f745a3ce8ff40e2ccaf1ad45db7774001b90d25810abd9040049be7bf4bb(s: Executing) returns (s': State)
+    ensures s'.ERROR?
+  {
+    return Revert(0, 0, s);
+  }
+
+  method revert_error_dbdddcbe895c83990c08b3492a0e83918d802a52331272ac6fdb6a7c4aea3b1b(s: Executing) returns (s': State)
+    ensures s'.ERROR?
+  {
+    return Revert(0, 0, s);
+  }
+
+
+  method abi_decode_tuple_(headStart: u256, dataEnd: u256, s: Executing) returns (s': State)
+    requires -TWO_255 <= dataEnd as int - headStart as int < TWO_255
+    ensures headStart <= dataEnd ==> s' == s
+    ensures s'.EXECUTING? ==> s' == s
+  {
+    if SLt(Sub(dataEnd, headStart), 0) {
+      s' := revert_error_dbdddcbe895c83990c08b3492a0e83918d802a52331272ac6fdb6a7c4aea3b1b(s) ;
     }
+    return s;
+  }
 
-    // case 0x18160ddd /* "totalSupply()" */ {
-    //     returnUint(totalSupply())
-    // }
-    // case 0xa9059cbb /* "transfer(address,uint256)" */ {
-    //     transfer(decodeAsAddress(0), decodeAsUint(1))
-    //     returnTrue()
-    // }
-    // case 0x23b872dd /* "transferFrom(address,address,uint256)" */ {
-    //     transferFrom(decodeAsAddress(0), decodeAsAddress(1), decodeAsUint(2))
-    //     returnTrue()
-    // }
-    // case 0x095ea7b3 /* "approve(address,uint256)" */ {
-    //     approve(decodeAsAddress(0), decodeAsUint(1))
-    //     returnTrue()
-    // }
-    // case 0xdd62ed3e /* "allowance(address,address)" */ {
-    //     returnUint(allowance(decodeAsAddress(0), decodeAsAddress(1)))
-    // }
-    // case 0x40c10f19 /* "mint(address,uint256)" */ {
-    //     mint(decodeAsAddress(0), decodeAsUint(1))
-    //     returnTrue()
-    // }
-    case _ => return Revert(0, 0, s);
+  function shift_right_unsigned_dynamic(bits: u256, value: u256): (newValue: u256)
+    ensures bits == 0 ==> newValue == value
+  {
+    assume bits == 0 ==> Shr(bits, value) == value;
+    Shr(bits, value)
+  }
 
+  function cleanup_from_storage_t_uint256(value: u256): (cleaned: u256) 
+  {
+    value
+  }
+
+  function extract_from_storage_value_dynamict_uint256(slot_value: u256, offset: u256) : (value: u256)
+    requires offset as nat * 8 < TWO_256
+    // ensures value == 
+  {
+    var k := shift_right_unsigned_dynamic(Mul(offset, 8), slot_value);
+    cleanup_from_storage_t_uint256(k)
+  }
+
+  function read_from_storage_split_dynamic_t_uint256(slot: u256, offset: u256, s: Executing): (value: u256)
+    requires offset as nat * 8 < TWO_256
+    ensures offset == 0 ==> value == s.Load(slot)
+  {
+    extract_from_storage_value_dynamict_uint256(SLoad(slot, s), offset)
+  }
+
+
+  method getter_fun_totalSupply_3(s: Executing) returns (ret: u256)
+    ensures ret == s.Load(0)
+  {
+    var slot := 0;
+    var offset := 0;
+    ret := read_from_storage_split_dynamic_t_uint256(slot, offset, s);
+  }
+
+
+  method cleanup_t_uint256(value: u256) returns (cleaned: u256)
+    ensures cleaned == value
+  {
+    cleaned := value;
+  }
+
+  /**
+    *  Store value at address pos in Memory.
+    */
+  method abi_encode_t_uint256_to_t_uint256_fromStack(value: u256, pos: u256, s: Executing) returns (s': State)
+    requires s.MemSize() % 32 == 0
+    ensures s'.EXECUTING?
+    ensures s'.MemSize() % 32 == 0
+    ensures s'.MemSize() > pos as nat + 31
+    ensures s'.yul.context == s.yul.context
+    ensures s'.yul.world == s.yul.world
+    ensures Memory.ReadUint256(s'.yul.memory, pos as nat) == value
+  {
+    var k := cleanup_t_uint256(value);
+    s' := MStore(pos, k, s);
+  }
+
+  /**
+    *  Store value0 at address headStart in memory and return the 
+    *  next available? memory slot (23-bytes)
+    */
+  method abi_encode_tuple_t_uint256__to_t_uint256__fromStack(headStart: u256 , value0: u256, s: Executing) returns (tail: u256, s': State)
+    requires s.MemSize() % 32 == 0
+    requires headStart as nat + 32 < TWO_256
+    ensures s'.EXECUTING?
+    ensures s'.MemSize() % 32 == 0
+    ensures tail == headStart + 32
+    ensures headStart as nat + 31 < s'.MemSize()
+    ensures Memory.ReadUint256(s'.yul.memory, headStart as nat) == value0
+  {
+    tail := Add(headStart, 32);
+    s' := abi_encode_t_uint256_to_t_uint256_fromStack(value0,  Add(headStart, 0), s);
+  }
+
+// lemma foo(s: )
+
+  method external_fun_totalSupply_3(s: Executing) returns (s': State)
+    requires 4 <= CallDataSize(s) as nat < TWO_255 - 4
+    requires s.MemSize() % 32 == 0
+    ensures s'.ERROR? || s'.RETURNS?
+    ensures s'.RETURNS? ==> |s'.data| == 32
+    ensures s'.RETURNS? ==> ByteUtils.ReadUint256(s'.data, 0) == s.Load(0)
+    // ensures
+  {
+    if CallValue(s) > 0 {
+      //  Not payable
+      var s1 := revert_error_ca66f745a3ce8ff40e2ccaf1ad45db7774001b90d25810abd9040049be7bf4bb(s);
+      return s1;
+    } else {
+      //  CallValue(s) == 0
+      assert CallValue(s) == 0;
+      var s1 := abi_decode_tuple_(4, CallDataSize(s), s);
+      var ret_0 :=  getter_fun_totalSupply_3(s1);
+      assert ret_0 == s1.Load(0) == s.Load(0);
+      var memPos, s2 := allocate_unbounded(s1);
+      assume memPos as nat + 32 < TWO_256;
+      //  Store ret_0 in memory at location memPos'
+      var memEnd, s3 := abi_encode_tuple_t_uint256__to_t_uint256__fromStack(memPos , ret_0, s2);
+      assert Memory.ReadUint256(s3.yul.memory, memPos as nat) == ret_0;
+      var x := RETURNS(data := Memory.Slice(s3.yul.memory, memPos as nat, (memEnd - memPos) as nat));
+
+      assert ByteUtils.ReadUint256(x.data, 0) == Memory.ReadUint256(s3.yul.memory, memPos as nat) == s.Load(0);
+      //  Return with data = memory slice between memPos of length memEnd - memPos
+    //   return RETURNS(data := Memory.Slice(s2.yul.memory, memPos as nat, (memEnd - memPos) as nat));
+      return x;
+    }
 
   }
 
@@ -136,33 +288,33 @@ module ERC20 {
   // }
 
   /* -------- storage layout ---------- */
-  function ownerPos(): u256 { 0 }
+  //   function ownerPos(): u256 { 0 }
 
-  function totalSupplyPos(): u256  { 1 }
+  //   function totalSupplyPos(): u256  { 1 }
 
   /**
     *   Storage slot for an account.
     */
-  function AccountToStorageOffset(account: u256): u256
-    requires account as nat < TWO_256 - 0x1000
-  {
-    Add(0x1000, account)
-  }
+  //   function AccountToStorageOffset(account: u256): u256
+  //     requires account as nat < TWO_256 - 0x1000
+  //   {
+  //     Add(0x1000, account)
+  //   }
 
   /**   
     *  Storage slot of allowance for an account.
     */
-  function AllowanceStorageOffset(account: u256, spender: u256, s: Executing): (r:   (u256, State))
-    requires account as nat < TWO_256 - 0x1000
-    requires s.MemSize() % 32 == 0
-    ensures r.1.EXECUTING?
-    ensures r.1.MemSize() % 32 == 0
-  {
-    var offset := AccountToStorageOffset(account);
-    var s1 := MStore(0, offset, s);
-    var s2 := MStore(0x20, spender, s);
-    Keccak256(0, 0x40, s2)
-  }
+  //   function AllowanceStorageOffset(account: u256, spender: u256, s: Executing): (r:   (u256, State))
+  //     requires account as nat < TWO_256 - 0x1000
+  //     requires s.MemSize() % 32 == 0
+  //     ensures r.1.EXECUTING?
+  //     ensures r.1.MemSize() % 32 == 0
+  //   {
+  //     var offset := AccountToStorageOffset(account);
+  //     var s1 := MStore(0, offset, s);
+  //     var s2 := MStore(0x20, spender, s);
+  //     Keccak256(0, 0x40, s2)
+  //   }
 
   /* -------- storage access ---------- */
   // function owner() -> o {
@@ -174,11 +326,11 @@ module ERC20 {
   // function mintTokens(amount) {
   //     sstore(totalSupplyPos(), safeAdd(totalSupply(), amount))
   // }
-  function balanceOf(account: u256, s: Executing): u256
-    requires account as nat < TWO_256 - 0x1000
-  {
-    SLoad(AccountToStorageOffset(account), s)
-  }
+  //   function balanceOf(account: u256, s: Executing): u256
+  //     requires account as nat < TWO_256 - 0x1000
+  //   {
+  //     SLoad(AccountToStorageOffset(account), s)
+  //   }
   // function addToBalance(account, amount) {
   //     let offset := accountToStorageOffset(account)
   //     sstore(offset, safeAdd(sload(offset), amount))
